Refactor join

join.v
@@ -1,4 +1,5 @@
-From WR Require Import syntax imports.
+From WR Require Import imports.
+Require Export Setoid.
 
 Definition is_bool_val a :=
   match a with
@@ -6,7 +7,6 @@ Definition is_bool_val a :=
   | tFalse => true
   | _ => false
   end.
-
 
 (* ------------------------------------------------------------ *)
 
@@ -21,7 +21,6 @@ Definition is_bool_val a :=
    confluence for its reflexive-transitive closure "⇒*".
 
  *)
-
 Reserved Infix "⇒" (at level 60, right associativity).
 Inductive Par : tm -> tm -> Prop :=
 | P_Var i :
@@ -51,7 +50,7 @@ Inductive Par : tm -> tm -> Prop :=
   a ⇒ tAbs a0 ->
   b0 ⇒ b1 ->
   (* ---------------------------- *)
-  tApp a b0 ⇒ (subst_tm (b1..) a0)
+  tApp a b0 ⇒ a0[b1..]
 | P_True :
   (* ------- *)
   tTrue ⇒ tTrue
@@ -77,34 +76,38 @@ Inductive Par : tm -> tm -> Prop :=
   (* ---------- *)
   tIf a b0 c0 ⇒ c1
 | P_Bool :
+  (* ---------- *)
   tBool ⇒ tBool
 | P_Refl :
+  (* ---------- *)
   tRefl ⇒ tRefl
 | P_Eq a0 b0 A0 a1 b1 A1 :
   a0 ⇒ a1 ->
   b0 ⇒ b1 ->
   A0 ⇒ A1 ->
+  (* ----------------------- *)
   tEq a0 b0 A0 ⇒ tEq a1 b1 A1
 | P_J t0 a0 b0 p0 t1 a1 b1 p1 :
   t0 ⇒ t1 ->
   a0 ⇒ a1 ->
   b0 ⇒ b1 ->
   p0 ⇒ p1 ->
+  (* ----------------------- *)
   tJ t0 a0 b0 p0 ⇒ tJ t1 a1 b1 p1
 | P_JRefl t0 a0 b0 p t1 a1 b1 :
   t0 ⇒ t1 ->
   a0 ⇒ a1 ->
   b0 ⇒ b1 ->
   p ⇒ tRefl ->
+  (* ------------------ *)
   tJ t0 a0 b0 p ⇒ t1
 | P_AbsEta a0 a1 :
   a0 ⇒ a1 ->
-  tAbs (tApp (ren_tm shift a0) (var_tm var_zero)) ⇒ a1
+  (* -------------------------------------- *)
+  tAbs (tApp a0⟨↑⟩ (var_tm var_zero)) ⇒ a1
 where "A ⇒ B" := (Par A B).
 
 #[export]Hint Constructors Par : par.
-
-Notation Pars := (rtc Par).
 
 (* The reflexive, transitive closure of parallel reduction. *)
 
@@ -115,110 +118,49 @@ Infix "⇒*" := (rtc Par) (at level 60, right associativity).
 Definition Coherent a0 a1 := (exists b, a0 ⇒* b /\ a1 ⇒* b).
 Infix "⇔" := Coherent (at level 70, no associativity).
 
+(* ------------------------------------------------------------ *)
+
+(* Parallel reduction is reflexive *)
+
+Lemma Par_refl (a : tm) : a ⇒ a.
+Proof. elim : a; hauto lq:on ctrs:Par. Qed.
+
+(* Parallel reduction is contained in Coherent *)
+
+Lemma Par_Coherent a b :
+  (a ⇒ b) -> Coherent a b.
+Proof. hauto lq:on use:@rtc_once, @rtc_refl. Qed.
+
+
+(* ------------------------------------------------------------ *)
+
+(* A top-level beta-reduction is a parallel reduction *)
+Lemma P_AppAbs_cbn (a b b0 : tm) :
+  b0 = a [b..] ->
+  (tApp (tAbs a) b) ⇒ b0.
+Proof. hauto lq:on ctrs:Par use:Par_refl. Qed.
+
+(* convenience introduction form for P_AppAbs',Eta' *)
+Lemma P_AppAbs' a a0 b0 b b1 :
+  b = a0 [b1..] ->
+  (a ⇒ tAbs a0) ->
+  (b0 ⇒ b1) ->
+  (* ---------------------------- *)
+  (tApp a b0) ⇒ b.
+Proof. hauto lq:on use:P_AppAbs. Qed.
+
 Lemma P_AbsEta' b a0 a1 :
   b = (tAbs (tApp (ren_tm shift a0) (var_tm var_zero))) ->
   Par a0 a1 ->
   Par b a1.
 Proof. move => ->. apply P_AbsEta. Qed.
 
-Lemma pars_pi_inv A B C (h : Pars (tPi A B) C) :
-  exists A0 B0, C = tPi A0 B0 /\ Pars A A0 /\ Pars B B0.
-Proof.
-  move E : (tPi A B) h => T h.
-  move : A B E.
-  elim : T C / h; hecrush inv:Par ctrs:Par, rtc.
-Qed.
-
-Lemma pars_eq_inv a b A C (h : Pars (tEq a b A) C) :
-  exists a0 b0 A0, C = tEq a0 b0 A0 /\ Pars a a0 /\ Pars b b0 /\ Pars A A0.
-Proof.
-  move E : (tEq a b A) h => T h.
-  move : a b A E.
-  elim : T C / h; hecrush inv:Par ctrs:Par, rtc.
-Qed.
-
-Lemma Coherent_pi_inj A B A0 B0 (h : Coherent (tPi A B) (tPi A0 B0)) :
-  Coherent A A0 /\ Coherent B B0.
-Proof. hauto q:on use:pars_pi_inv. Qed.
-
-Lemma Coherent_eq_inj a b A a0 b0 A0 (h : Coherent (tEq a b A) (tEq a0 b0 A0)) : Coherent a a0 /\ Coherent b b0 /\ Coherent A A0.
-Proof. hauto q:on use:pars_eq_inv. Qed.
-
-Lemma pars_univ_inv i A (h : Pars (tUniv i) A) :
-  A = tUniv i.
-Proof.
-  move E : (tUniv i) h => A0 h.
-  move : E.
-  elim : A0 A / h; hauto lq:on rew:off ctrs:rtc, Par inv:Par.
-Qed.
-
-Lemma Coherent_univ_inj i j (h : Coherent (tUniv i) (tUniv j)) : i = j.
-Proof. hauto lq:on rew:off inv:rtc use:pars_univ_inv. Qed.
-
 (* ------------------------------------------------------------ *)
 
-(* Parallel reduction is reflexive *)
+(* Par (⇒), Pars (⇒* ), and ⇔ are closed under renaming *)
 
-Lemma Par_refl (a : tm) : Par a a.
-Proof. elim : a; hauto lq:on ctrs:Par. Qed.
-
-Lemma P_AppAbs_cbn (a b b0 : tm) :
-  b0 = subst_tm (b..) a ->
-  Par (tApp (tAbs a) b) b0.
-Proof. hauto lq:on ctrs:Par use:Par_refl. Qed.
-
-Lemma P_IfTrue_star a b c :
-  Pars a tTrue ->
-  Pars (tIf a b c) b.
-  move E : tTrue => v h.
-  move : E.
-  elim : a v / h.
-  - hauto lq:on ctrs:Par use:Par_refl, @rtc_once.
-  - move => a a0 a1 h0 h1 h2 ?; subst.
-    move /(_ eq_refl) in h2.
-    apply : rtc_transitive; eauto.
-    hauto lq:on use:@rtc_once,Par_refl ctrs:Par.
-Qed.
-
-Lemma P_IfFalse_star a b c :
-  Pars a tFalse ->
-  Pars (tIf a b c) c.
-  move E : tFalse => v h.
-  move : E.
-  elim : a v / h.
-  - hauto lq:on ctrs:Par use:Par_refl, @rtc_once.
-  - move => a a0 a1 h0 h1 h2 ?; subst.
-    move /(_ eq_refl) in h2.
-    apply : rtc_transitive; eauto.
-    apply @rtc_once.
-    hauto lq:on ctrs:Par use:Par_refl.
-Qed.
-
-Lemma P_JRefl_star t a b p :
-  Pars p tRefl  ->
-  Pars (tJ t a b p) t.
-Proof.
-  move E : tRefl => v h.
-  move : E.
-  elim : p v / h.
-  - hauto lq:on ctrs:Par use:Par_refl, @rtc_once.
-  - move => x y z h0 h1 ih ?; subst.
-    move /(_ ltac:(done)) in ih.
-    apply : rtc_l; eauto.
-    apply P_J; sfirstorder use:Par_refl.
-Qed.
-
-Lemma P_AppAbs' a a0 b0 b b1 :
-  b = subst_tm (b1..) a0 ->
-  Par a (tAbs a0) ->
-  Par b0 b1 ->
-  (* ---------------------------- *)
-  Par (tApp a b0) b.
-Proof. hauto lq:on use:P_AppAbs. Qed.
-
-Lemma par_renaming a b (ξ : fin -> fin) :
-  Par a b ->
-  Par (ren_tm ξ a) (ren_tm ξ b).
+Lemma Par_renaming a b (ξ : fin -> fin) :
+  (a ⇒ b) -> (a⟨ξ⟩ ⇒ b⟨ξ⟩).
 Proof.
   move => h.
   move : ξ.
@@ -229,6 +171,312 @@ Proof.
     apply : P_AbsEta'; eauto. by asimpl.
 Qed.
 
+Lemma Pars_renaming a b (ξ : fin -> fin) :
+  (a ⇒* b) -> (a⟨ξ⟩ ⇒* b⟨ξ⟩).
+Proof. induction 1; hauto lq:on ctrs:rtc use:Par_renaming. Qed.
+
+Lemma Coherent_renaming a b (ξ : fin -> fin) :
+  Coherent a b ->
+  Coherent a⟨ξ⟩ b⟨ξ⟩.
+Proof. hauto lq:on rew:off use:Pars_renaming. Qed.
+
+Local Lemma Par_morphing_lift (ξ0 ξ1 : fin -> tm)
+  (h : forall i, (ξ0 i ⇒ ξ1 i)) :
+  forall i, (up_tm_tm ξ0 i ⇒ up_tm_tm ξ1 i).
+Proof. case => [|i]; first by constructor. asimpl. by apply Par_renaming. Qed.
+
+(* ------------------------------------------------------------ *)
+
+(* Now we want to show all of the ways that these relations are closed
+   under substitution. *)
+
+(* First, we extend the Par, Pars and Coherent relations to substitutions *)
+
+Definition Par_m (σ0 σ1 : fin -> tm) := (forall i, (σ0 i) ⇒ (σ1 i)).
+
+Infix "⇒ς"  := Par_m (at level 70, right associativity).
+Infix "⇒ς*" := (rtc Par_m) (at level 70, right associativity).
+
+Definition Coherent_m σ0 σ1 :=
+  exists σ, (σ0 ⇒ς* σ) /\ (σ1 ⇒ς* σ).
+
+(* Morphing lemmas *)
+(* TODO: make the names of these lemmas a little more meaningful? *)
+
+Lemma Par_morphing a b (σ0 σ1 : fin -> tm)
+  (h : σ0 ⇒ς σ1) :
+  (a ⇒ b) ->
+  (a[σ0] ⇒ b[σ1]).
+Proof.
+  move => h0.
+  move : σ0 σ1 h.
+  elim : a b / h0 => /=; eauto with par.
+  - hauto lq:on db:par use:Par_morphing_lift unfold:Par_m.
+  - hauto lq:on db:par use:Par_morphing_lift unfold:Par_m.
+  - move => *; apply : P_AppAbs'; eauto; by asimpl.
+  - hauto lq:on db:par use:Par_morphing_lift.
+  - hauto lq:on db:par use:Par_morphing_lift.
+  - move => *; apply : P_AbsEta'; eauto. by asimpl.
+Qed.
+
+Lemma Par_morphing_star a0 a1 (h : a0 ⇒* a1) (σ0 σ1 : fin -> tm) :
+  (σ0 ⇒ς σ1) ->
+  (a0[σ0] ⇒* a1 [σ1]).
+Proof.
+  induction h.
+  - move => h. apply @rtc_once. eauto using Par_morphing, Par_refl.
+  - move => h0.
+    apply : rtc_transitive; eauto.
+    apply @rtc_once.
+    sfirstorder use:Par_morphing, Par_refl.
+Qed.
+
+Lemma Coherent_morphing a0 a1 (h : Coherent a0 a1) (σ0 σ1 : fin -> tm) :
+  (σ0 ⇒ς σ1) ->
+  Coherent (a0[σ0]) (a1[σ1]).
+Proof.
+  hauto l:on use:Par_morphing_star, Par_refl,
+    Par_Coherent unfold:Coherent, Par_m.
+Qed.
+
+Lemma Pars_morphing a b (σ0 σ1 : fin -> tm)
+  (h : σ0 ⇒ς* σ1) :
+  (a ⇒ b) ->
+  (a [σ0]) ⇒* (b[σ1]).
+Proof.
+  move : a b.
+  elim : σ0 σ1 / h.
+  - sfirstorder unfold:Par_m use:Par_morphing, @rtc_once, Par_refl.
+  - hauto lq:on unfold:Par_m use:Par_morphing, Par_refl ctrs:rtc.
+Qed.
+
+
+Lemma Pars_morphing_star a b (σ0 σ1 : fin -> tm)
+  (h : σ0 ⇒ς* σ1)
+  (h0 : a ⇒* b) :
+  (a [σ0] ⇒* b[σ1]).
+Proof.
+  elim : a b / h0.
+  - sfirstorder use:Pars_morphing, Par_refl.
+  - move => x y z /[swap] _.
+    move : Pars_morphing (rtc_refl Par_m σ0); repeat move /[apply].
+    apply rtc_transitive.
+Qed.
+
+Lemma Coherent_morphing_star a b σ0 σ1
+  (h : Coherent_m σ0 σ1)
+  (h0 : Coherent a b) :
+  Coherent (a[σ0]) (b[σ1]).
+Proof.
+  hauto q:on use:Pars_morphing_star unfold:Coherent.
+Qed.
+
+
+
+(* These two lemmas allow us to create substitutions
+   that are related by paralell reduction. *)
+
+Lemma good_Pars_morphing_ext a b σ0 σ1
+  (h : a ⇒* b) :
+  (σ0 ⇒ς* σ1) ->
+  ((a .: σ0) ⇒ς* (b .: σ1)).
+Proof.
+  elim : a b /h.
+  - move => a.
+    move => h.
+    elim : σ0 σ1 / h; first by sfirstorder.
+    move => σ0 σ1 σ2 h h1.
+    apply rtc_transitive. apply rtc_once.
+    qauto l:on unfold:Par_m ctrs:rtc inv:nat use:Par_refl.
+  - move => x y z ha hb /[apply].
+    apply rtc_transitive. apply rtc_once.
+    hauto lq:on unfold:Par_m inv:nat use:Par_refl.
+Qed.
+
+Lemma good_Pars_morphing_ext2 a0 b0 a1 b1 σ0 σ1
+  (h : a0 ⇒* b0) (h1 : a1 ⇒*  b1) :
+  (σ0 ⇒ς* σ1) ->
+  ((a0 .: (a1 .: σ0)) ⇒ς* (b0 .: (b1 .: σ1))).
+Proof. sfirstorder use:good_Pars_morphing_ext. Qed.
+
+
+(* The three relations are closed under substitution *)
+
+Lemma Par_subst a0 a1 (h : a0 ⇒ a1) (σ : fin -> tm) :
+  (a0[σ] ⇒ a1[σ]).
+Proof. hauto l:on unfold:Par_m use:Par_refl, Par_morphing. Qed.
+
+Lemma Par_subst_star a0 a1 (h : a0 ⇒* a1) (σ : fin -> tm) :
+  (a0 [σ]) ⇒* (a1 [σ]).
+Proof. hauto l:on use:Par_morphing_star, Par_refl unfold:Par_m. Qed.
+
+Lemma Coherent_subst_star a0 a1 (h : Coherent a0 a1) (σ : fin -> tm) :
+  Coherent (a0[σ]) (a1 [σ]).
+Proof. hauto lq:on use:Coherent_morphing, Par_refl unfold:Par_m. Qed.
+
+
+(* The relations are also closed under single substitution  *)
+
+(* TODO: is _cong the right name for these lemmas? *)
+
+Lemma Par_cong a0 a1 b0 b1 (h : a0 ⇒ a1) (h1 : b0 ⇒ b1) :
+  (a0 [b0..] ⇒ a1 [b1..]).
+Proof.
+  apply Par_morphing; auto.
+  case; auto.
+  sfirstorder use:Par_refl.
+Qed.
+
+
+Local Lemma Coherent_cong_helper : forall a0 c, (a0 ⇒* c) -> (a0.. ⇒ς* c..).
+Proof.
+  move => a0 c h2.
+  elim : a0 c / h2.
+    sfirstorder.
+    move => a b c ? ?.
+    apply rtc_transitive with (y := b..).
+    sauto lq:on unfold:Par_m inv:nat use:Par_refl use:good_Pars_morphing_ext.
+Qed.
+
+Lemma Coherent_cong a0 a1 b0 b1
+  (h : Coherent a0 a1)
+  (h1 : Coherent b0 b1) :
+  Coherent (a0 [b0..]) (a1 [b1..]).
+Proof.
+  apply Coherent_morphing_star=>//.
+  sfirstorder use:Coherent_cong_helper.
+Qed.
+
+
+
+
+(* ------------------------------------------------------------ *)
+
+(* Inversion lemmas *)
+
+Lemma Pars_pi_inv A B C (h : (tPi A B) ⇒* C) :
+  exists A0 B0, C = tPi A0 B0 /\ (A ⇒* A0) /\ (B ⇒* B0).
+Proof.
+  move E : (tPi A B) h => T h.
+  move : A B E.
+  elim : T C / h; hecrush inv:Par ctrs:Par, rtc.
+Qed.
+
+Lemma Pars_eq_inv a b A C (h : (tEq a b A) ⇒* C) :
+  exists a0 b0 A0, C = tEq a0 b0 A0 /\ a ⇒* a0 /\ b ⇒* b0 /\ A ⇒* A0.
+Proof.
+  move E : (tEq a b A) h => T h.
+  move : a b A E.
+  elim : T C / h; hecrush inv:Par ctrs:Par, rtc.
+Qed.
+
+Lemma Coherent_pi_inj A B A0 B0 (h : Coherent (tPi A B) (tPi A0 B0)) :
+  Coherent A A0 /\ Coherent B B0.
+Proof. hauto q:on use:Pars_pi_inv. Qed.
+
+Lemma Coherent_eq_inj a b A a0 b0 A0 (h : Coherent (tEq a b A) (tEq a0 b0 A0)) : Coherent a a0 /\ Coherent b b0 /\ Coherent A A0.
+Proof. hauto q:on use:Pars_eq_inv. Qed.
+
+Lemma Pars_univ_inv i A (h : (tUniv i) ⇒* A) :
+  A = tUniv i.
+Proof.
+  move E : (tUniv i) h => A0 h.
+  move : E.
+  elim : A0 A / h; hauto lq:on rew:off ctrs:rtc, Par inv:Par.
+Qed.
+
+Lemma Coherent_univ_inj i j (h : Coherent (tUniv i) (tUniv j)) : i = j.
+Proof. hauto lq:on rew:off inv:rtc use:Pars_univ_inv. Qed.
+
+
+(* ------------------------------------------------------------ *)
+
+
+Lemma P_IfTrue_star a b c :
+  (a ⇒* tTrue) ->
+  ((tIf a b c) ⇒* b).
+  move E : tTrue => v h.
+  move : E.
+  elim : a v / h.
+  - move => *. subst.
+    apply rtc_once. apply : P_IfTrue; apply Par_refl.
+  - move => a a0 a1 h0 h1 h2 ?; subst.
+    move /(_ eq_refl) in h2.
+    apply : rtc_transitive; eauto.
+    hauto lq:on use:@rtc_once,Par_refl ctrs:Par.
+Qed.
+
+Lemma P_IfFalse_star a b c :
+  (a ⇒* tFalse) ->
+  ((tIf a b c) ⇒* c).
+  move E : tFalse => v h.
+  move : E.
+  elim : a v / h.
+  - move => *. subst.
+    apply rtc_once. apply : P_IfFalse; apply Par_refl.
+  - move => a a0 a1 h0 h1 h2 ?; subst.
+    move /(_ eq_refl) in h2.
+    apply : rtc_transitive; eauto.
+    apply @rtc_once.
+    hauto lq:on ctrs:Par use:Par_refl.
+Qed.
+
+Lemma P_JRefl_star t a b p :
+  (p ⇒* tRefl)  ->
+  ((tJ t a b p) ⇒* t).
+Proof.
+  move E : tRefl => v h.
+  move : E.
+  elim : p v / h.
+  - move => *. subst.
+    apply rtc_once. apply : P_JRefl; apply Par_refl.
+  - move => x y z h0 h1 ih ?; subst.
+    move /(_ ltac:(done)) in ih.
+    apply : rtc_l; eauto.
+    apply P_J; sfirstorder use:Par_refl.
+Qed.
+
+
+(* ------------------------------------------------------------ *)
+
+(* Derived inversion principle for "Par" that doesn't
+   generate free names with use. *)
+Derive Inversion Par_inv with (forall a b, a ⇒ b).
+
+(* Induction metric for terms  *)
+Definition size_tm : tm -> nat.
+  apply tm_rec.
+  exact (fun _ => 1).
+  exact (fun _ a => 1 + a).
+  exact (fun _ a _ b => 1 + a + b).
+  exact (fun _ a _ b => 1 + a + b).
+  exact 1.
+  exact (fun _ => 1).
+  exact 1.
+  exact 1.
+  exact (fun _ a _ b _ c => 1 + a + b + c).
+  exact 1.
+  exact (fun _ a _ b _ c => 1 + a + b + c).
+  exact (fun _ a _ b _ c _ d => 1 + a + b + c + d).
+  exact 1.
+Defined.
+
+Lemma ren_tm_size_tm a ξ : size_tm a = size_tm (ren_tm ξ a).
+Proof. elim : a ξ; scongruence. Qed.
+
+Lemma induction_size_tm_lt
+  : forall P : tm -> Prop,
+       (forall x : tm, (forall y : tm, size_tm y < size_tm x -> P y) -> P x) ->
+       forall a : tm, P a.
+Proof.
+  have := well_founded_ltof  tm size_tm.
+  move => + + + a.
+  move /(_ a). elim; hauto lq:on.
+Qed.
+
+Local Ltac apply_ih ih := move /ih; elim; last by (simpl; lia).
+
+(* Characterization of variable freeness conditions *)
 Definition tm_i_free a i := exists ξ ξ0, ξ i <> ξ0 i /\ ren_tm ξ a = ren_tm ξ0 a.
 
 Lemma subst_differ_one_ren_up i ξ0 ξ1 :
@@ -261,40 +509,6 @@ Proof.
   - hauto lq:on rew:off.
   - hauto lq:on rew:off.
 Qed.
-
-Definition size_tm : tm -> nat.
-  apply tm_rec.
-  exact (fun _ => 1).
-  exact (fun _ a => 1 + a).
-  exact (fun _ a _ b => 1 + a + b).
-  exact (fun _ a _ b => 1 + a + b).
-  exact 1.
-  exact (fun _ => 1).
-  exact 1.
-  exact 1.
-  exact (fun _ a _ b _ c => 1 + a + b + c).
-  exact 1.
-  exact (fun _ a _ b _ c => 1 + a + b + c).
-  exact (fun _ a _ b _ c _ d => 1 + a + b + c + d).
-  exact 1.
-Defined.
-
-Lemma ren_tm_size_tm a ξ : size_tm a = size_tm (ren_tm ξ a).
-Proof. elim : a ξ; scongruence. Qed.
-
-Lemma induction_size_tm_lt
-  : forall P : tm -> Prop,
-       (forall x : tm, (forall y : tm, size_tm y < size_tm x -> P y) -> P x) ->
-       forall a : tm, P a.
-Proof.
-  have := well_founded_ltof  tm size_tm.
-  move => + + + a.
-  move /(_ a). elim; hauto lq:on.
-Qed.
-
-Derive Inversion Par_inv with (forall a b, Par a b).
-
-Local Ltac apply_ih ih := move /ih; elim; last by (simpl; lia).
 
 (* ------------------ antirenaming ------------------------- *)
 
@@ -403,168 +617,11 @@ Proof.
   - hauto lq:on dep:on inv:Par ctrs:Par.
 Qed.
 
-Lemma pars_renaming a b (ξ : fin -> fin) :
-  Pars a b ->
-  Pars (ren_tm ξ a) (ren_tm ξ b).
-Proof. induction 1; hauto lq:on ctrs:rtc use:par_renaming. Qed.
+(* ------------------------------------------------------------ *)
 
-Lemma Coherent_renaming a b (ξ : fin -> fin) :
-  Coherent a b ->
-  Coherent (ren_tm ξ a) (ren_tm ξ b).
-Proof. hauto lq:on rew:off use:pars_renaming. Qed.
-
-Lemma par_morphing_lift (ξ0 ξ1 : fin -> tm)
-  (h : forall i, Par (ξ0 i) (ξ1 i)) :
-  forall i, Par (up_tm_tm ξ0 i) (up_tm_tm ξ1 i).
-Proof.
-  case => [|i]; first by constructor.
-  asimpl.
-  by apply par_renaming.
-Qed.
-
-Lemma par_morphing a b (ξ0 ξ1 : fin -> tm)
-  (h : forall i, Par (ξ0 i) (ξ1 i)) :
-  Par a b ->
-  Par (subst_tm ξ0 a) (subst_tm ξ1 b).
-Proof.
-  move => h0.
-  move : ξ0 ξ1 h.
-  elim : a b / h0 => /=; eauto with par.
-  - hauto lq:on db:par use:par_morphing_lift.
-  - hauto lq:on db:par use:par_morphing_lift.
-  - move => *; apply : P_AppAbs'; eauto; by asimpl.
-  - hauto lq:on db:par use:par_morphing_lift.
-  - hauto lq:on db:par use:par_morphing_lift.
-  - move => *; apply : P_AbsEta'; eauto. by asimpl.
-Qed.
-
-Inductive good_Pars_morphing : (fin -> tm) -> (fin -> tm) -> Prop :=
-| good_Pars_morphing_one ξ :
-  good_Pars_morphing ξ ξ
-| good_Pars_morphing_cons ξ0 ξ1 ξ2 :
-  (forall i, Par (ξ0 i) (ξ1 i)) ->
-  good_Pars_morphing ξ1 ξ2 ->
-  good_Pars_morphing ξ0 ξ2.
-
-Lemma good_Pars_morphing_ext a b ξ0 ξ1
-  (h : Pars a b) :
-  good_Pars_morphing ξ0 ξ1 ->
-  good_Pars_morphing (a .: ξ0) (b .: ξ1).
-Proof.
-  elim : a b /h.
-  - move => a.
-    move => h.
-    elim : ξ0 ξ1 / h; first by sfirstorder.
-    move => ξ0 ξ1 ξ2 h h1.
-    apply good_Pars_morphing_cons.
-    hauto lq:on inv:nat use:Par_refl.
-  - move => x y z ha hb /[apply].
-    apply : good_Pars_morphing_cons.
-    hauto lq:on inv:nat use:Par_refl.
-Qed.
-
-Lemma good_Pars_morphing_ext2 a0 b0 a1 b1 ξ0 ξ1
-  (h : Pars a0 b0) (h1 : Pars a1 b1) :
-  good_Pars_morphing ξ0 ξ1 ->
-  good_Pars_morphing (a0 .: (a1 .: ξ0)) (b0 .: (b1 .: ξ1)).
-Proof. sfirstorder use:good_Pars_morphing_ext. Qed.
-
-(* No idea how to induct on (forall i, Pars (ξ0 i) (ξ1 i) ) *)
-Lemma Pars_morphing a b (ξ0 ξ1 : fin -> tm)
-  (h : good_Pars_morphing ξ0 ξ1) :
-  Par a b ->
-  Pars (subst_tm ξ0 a) (subst_tm ξ1 b).
-Proof.
-  move : a b.
-  elim : ξ0 ξ1 / h.
-  - sfirstorder use:par_morphing, @rtc_once, Par_refl.
-  - hauto lq:on use:par_morphing, Par_refl ctrs:rtc.
-Qed.
-
-Lemma Pars_morphing_star a b (ξ0 ξ1 : fin -> tm)
-  (h : good_Pars_morphing ξ0 ξ1)
-  (h0 : Pars a b) :
-  Pars (subst_tm ξ0 a) (subst_tm ξ1 b).
-Proof.
-  elim : a b / h0.
-  - sfirstorder use:Pars_morphing, Par_refl.
-  - move => x y z /[swap] _.
-    move : Pars_morphing (good_Pars_morphing_one ξ0); repeat move /[apply].
-    apply rtc_transitive.
-Qed.
-
-Definition good_coherent_morphing ξ0 ξ1 :=
-  exists ξ, good_Pars_morphing ξ0 ξ /\ good_Pars_morphing ξ1 ξ.
-
-Lemma coherent_morphing_star a b ξ0 ξ1
-  (h : good_coherent_morphing ξ0 ξ1)
-  (h0 : Coherent a b) :
-  Coherent (subst_tm ξ0 a) (subst_tm ξ1 b).
-Proof.
-  hauto q:on use:Pars_morphing_star unfold:Coherent.
-Qed.
-
-Lemma coherent_cong_helper : forall a0 c, Pars a0 c -> good_Pars_morphing a0.. c.. .
-Proof.
-  move => a0 c h2.
-  elim : a0 c / h2.
-    sfirstorder.
-    move => a b c ? ?.
-    apply : good_Pars_morphing_cons.
-    hauto lq:on inv:nat use:Par_refl.
-Qed.
-
-Lemma coherent_cong a0 a1 b0 b1
-  (h : Coherent a0 b0)
-  (h1 : Coherent a1 b1) :
-  Coherent (subst_tm (a0..) a1) (subst_tm (b0..) b1).
-Proof.
-  apply coherent_morphing_star=>//.
-  sfirstorder use:coherent_cong_helper.
-Qed.
-
-Lemma Par_cong a0 a1 b0 b1 (h : Par a0 a1) (h1 : Par b0 b1) :
-  Par (subst_tm (b0..) a0) (subst_tm (b1..) a1).
-Proof.
-  apply par_morphing; auto.
-  case; auto.
-  sfirstorder use:Par_refl.
-Qed.
-
-Lemma Par_subst a0 a1 (h : Par a0 a1) (ξ : fin -> tm) :
-  Par (subst_tm ξ a0) (subst_tm ξ a1).
-Proof. hauto l:on use:Par_refl, par_morphing. Qed.
-
-Lemma par_morphing_star a0 a1 (h : Pars a0 a1) (ξ0 ξ1 : fin -> tm) :
-  (forall i, Par (ξ0 i) (ξ1 i)) ->
-  Pars (subst_tm ξ0 a0) (subst_tm ξ1 a1).
-Proof.
-  induction h.
-  - move => h. apply @rtc_once. eauto using par_morphing, Par_refl.
-  - move => h0.
-    apply : rtc_transitive; eauto.
-    apply @rtc_once.
-    sfirstorder use:par_morphing, Par_refl.
-Qed.
-
-Lemma Par_Coherent a b :
-  Par a b -> Coherent a b.
-Proof. hauto lq:on use:@rtc_once, @rtc_refl. Qed.
-
-Lemma Coherent_morphing a0 a1 (h : Coherent a0 a1) (ξ0 ξ1 : fin -> tm) :
-  (forall i, Par (ξ0 i) (ξ1 i)) ->
-  Coherent (subst_tm ξ0 a0) (subst_tm ξ1 a1).
-Proof.
-  hauto l:on use:par_morphing_star, Par_refl, Par_Coherent unfold:Coherent.
-Qed.
-
-Lemma Par_subst_star a0 a1 (h : Pars a0 a1) (ξ : fin -> tm) :
-  Pars (subst_tm ξ a0) (subst_tm ξ a1).
-Proof. hauto l:on use:par_morphing_star, Par_refl. Qed.
-
-Lemma Coherent_subst_star a0 a1 (h : Coherent a0 a1) (ξ : fin -> tm) :
-  Coherent (subst_tm ξ a0) (subst_tm ξ a1).
-Proof. hauto lq:on use:Coherent_morphing, Par_refl. Qed.
+(* We want to show that Coherent is an equivalence relation. But,
+   to show that it is transitive, we need to show that parallel
+   reduction is confluent. *)
 
 Local Ltac apply_ih' ih :=
   move :(ih); repeat move/[apply]; elim;
@@ -573,6 +630,7 @@ Local Ltac apply_ih' ih :=
 Local Ltac apply_ih'' ih :=
   move /ih; move /(_ ltac:(simpl; lia)).
 
+(* Simple helper function *)
 Lemma par_var_eq i a : Par (var_tm i) a -> a = var_tm i.
 Proof. elim /Par_inv=>//. Qed.
 
@@ -690,10 +748,12 @@ Proof.
       move : h1 h3. apply_ih' ih. eauto.
 Qed.
 
-Lemma pars_confluent : confluent Par.
+Lemma Pars_confluent : confluent Par.
 Proof.
   sfirstorder use:Par_confluent, @diamond_confluent.
 Qed.
+
+(* Coherent is an equivalence relation *)
 
 Lemma Coherent_reflexive a :
   Coherent a a.
@@ -706,7 +766,7 @@ Proof. sfirstorder. Qed.
 Lemma Coherent_transitive a b c :
   Coherent a b -> Coherent b c -> Coherent a c.
 Proof.
-  have := pars_confluent.
+  have := Pars_confluent.
   move => h [z0 [? h0]] [z1 [h1 ?]].
   move /(_ b _ _ h0 h1) in h.
   case : h => z [*].
