typing.v
@@ -1,4 +1,16 @@
-From WR Require Import imports join common.
+From WR Require Import imports join.
+
+Definition context := list tm.
+
+Inductive lookup : nat -> context -> tm -> Prop :=
+  | here : forall {A Γ}, lookup 0 (A :: Γ) (A ⟨shift⟩)
+  | there : forall {n A Γ B},
+      lookup n Γ A -> lookup (S n) (B :: Γ) (A ⟨shift⟩).
+
+Definition lookup_good_renaming ξ Γ Δ :=
+  forall i A, lookup i Γ A -> lookup (ξ i) Δ A⟨ξ⟩.
+
+Derive Inversion lookup_inv with (forall i Γ A, lookup i Γ A).
 
 Reserved Notation "Γ ⊢ a ∈ A" (at level 70).
 Reserved Notation "⊢ Γ" (at level 70).
